Compiler.thy
@@ -9,6 +9,35 @@ abbreviation code_compile :: "texpr \<Rightarrow> mach list" where
 abbreviation compile :: "nexpr \<rightharpoonup> mach list" where 
   "compile \<equiv> map_option (code_compile \<circ> fst) \<circ> typecheck"
 
+primrec quick_convert :: "var set \<Rightarrow> nexpr \<Rightarrow> hexpr \<times> var set" where
+  "quick_convert vs (NVar x) = (HVar x, vs)"
+| "quick_convert vs (NConst k) = (hexpr.HConst k, vs)"
+| "quick_convert vs (NLam x e) = (
+    let v = fresh vs
+    in let (e', vs') = quick_convert (insert v vs) e
+    in (hexpr.HLam x (Var v) e', vs'))"
+| "quick_convert vs (NApp e\<^sub>1 e\<^sub>2) = (
+    let v = fresh vs
+    in let (e\<^sub>1', vs') = quick_convert (insert v vs) e\<^sub>1 
+    in let (e\<^sub>2', vs'') = quick_convert vs' e\<^sub>2 
+    in (HApp e\<^sub>1' e\<^sub>2', vs''))"
+
+primrec collect_constraints :: "subst \<Rightarrow> var set \<Rightarrow> nexpr \<Rightarrow> uexpr \<times> var set \<times> (uexpr \<times> uexpr) list" 
+    where
+  "collect_constraints \<Gamma> vs (NVar x) = (case \<Gamma> x of 
+      Some t \<Rightarrow> (t, vs, []) 
+    | None \<Rightarrow> (undefined, vs, fail))"
+| "collect_constraints \<Gamma> vs (NConst k) = (Ctor ''Base'' [], vs, [])"
+| "collect_constraints \<Gamma> vs (NLam x e) = (
+    let v = fresh vs
+    in let (t, vs', con) = collect_constraints (\<Gamma>(x \<mapsto> Var v)) (insert v vs) e
+    in (Ctor ''Arrow'' [Var v, t], vs', con))"
+| "collect_constraints \<Gamma> vs (NApp e\<^sub>1 e\<^sub>2) = (
+    let v = fresh vs
+    in let (t\<^sub>1, vs', con\<^sub>1) = collect_constraints \<Gamma> (insert v vs) e\<^sub>1 
+    in let (t\<^sub>2, vs'', con\<^sub>2) = collect_constraints \<Gamma> vs' e\<^sub>2 
+    in (Var v, vs'', (t\<^sub>1, Ctor ''Arrow'' [t\<^sub>2, Var v]) # con\<^sub>1 @ con\<^sub>2))"
+
 primrec tree_code_size :: "tree_code \<Rightarrow> nat"
     and tree_code_size_list :: "tree_code list \<Rightarrow> nat" where
   "tree_code_size (TLookup x) = 0"
@@ -19,11 +48,11 @@ primrec tree_code_size :: "tree_code \<Rightarrow> nat"
 | "tree_code_size_list (op # cd) = 
       Suc (if op = TApply \<and> cd = [] then 0 else tree_code_size op + tree_code_size_list cd)"
 
-primrec alg_compile1 :: "var list \<Rightarrow> texpr \<Rightarrow> tree_code list \<Rightarrow> tree_code list" where
-  "alg_compile1 \<Phi> (texpr.TVar x) acc = TLookup (the (idx_of \<Phi> x)) # acc"
-| "alg_compile1 \<Phi> (texpr.TConst k) acc = TPushCon k # acc"
-| "alg_compile1 \<Phi> (texpr.TLam x t e) acc = TPushLam (alg_compile1 (insert_at 0 x \<Phi>) e []) # acc"
-| "alg_compile1 \<Phi> (texpr.TApp e\<^sub>1 e\<^sub>2) acc = alg_compile1 \<Phi> e\<^sub>1 (alg_compile1 \<Phi> e\<^sub>2 (TApply # acc))"
+primrec alg_compile1 :: "var list \<Rightarrow> nexpr \<Rightarrow> tree_code list \<Rightarrow> tree_code list" where
+  "alg_compile1 \<Phi> (NVar x) acc = TLookup (the (idx_of \<Phi> x)) # acc"
+| "alg_compile1 \<Phi> (NConst k) acc = TPushCon k # acc"
+| "alg_compile1 \<Phi> (NLam x e) acc = TPushLam (alg_compile1 (insert_at 0 x \<Phi>) e []) # acc"
+| "alg_compile1 \<Phi> (NApp e\<^sub>1 e\<^sub>2) acc = alg_compile1 \<Phi> e\<^sub>1 (alg_compile1 \<Phi> e\<^sub>2 (TApply # acc))"
 
 function alg_compile2 :: "nat \<Rightarrow> tree_code list \<Rightarrow> byte_code list \<Rightarrow> byte_code list" where
   "alg_compile2 lib [] acc = BReturn # acc"
@@ -39,11 +68,32 @@ function alg_compile2 :: "nat \<Rightarrow> tree_code list \<Rightarrow> byte_co
 termination
   by (relation "measure (tree_code_size_list \<circ> fst \<circ> snd)") simp_all
 
-definition alg_compile :: "texpr \<Rightarrow> byte_code list" where
-  "alg_compile e = alg_compile2 0 (alg_compile1 [] e []) []"
+definition alg_compile :: "nexpr \<rightharpoonup> byte_code list" where
+  "alg_compile e = (
+    let (t, vs, con) = collect_constraints Map.empty {} e
+    in if unify' con \<noteq> None then Some (alg_compile2 0 (alg_compile1 [] e []) []) else None)"
 
-lemma [simp]: "alg_compile1 \<Phi> e acc = encode (convert' \<Phi> e) @ acc"
-  by (induction e arbitrary: \<Phi> acc) simp_all
+lemma [simp]: "encode (convert' \<Phi> (tsubstt sub e)) = encode (convert' \<Phi> e)"
+  by (induction e arbitrary: \<Phi>) simp_all
+
+lemma [simp]: "encode \<circ> convert \<circ> tsubstt sub = encode \<circ> convert"
+  by (auto simp add: convert_def)
+
+lemma [simp]: "typecheck' \<Gamma> vs e = (e', t, vs', con) \<Longrightarrow> quick_convert vs e = (e', vs')"
+  by (induction e arbitrary: \<Gamma> vs e' t vs' con) 
+     (simp_all add: Let_def split: option.splits prod.splits)
+
+lemma [simp]: "quick_convert vs e = (e', vs') \<Longrightarrow> 
+    alg_compile1 \<Phi> e acc = encode (convert' \<Phi> (solidify e')) @ acc"
+  by (induction e arbitrary: \<Phi> acc vs e' vs') (auto simp add: Let_def split: prod.splits)
+
+lemma [simp]: "typecheck' \<Gamma> vs e = (e', t, vs', con) \<Longrightarrow> 
+  alg_compile1 \<Phi> e acc = encode (convert' \<Phi> (solidify e')) @ acc"
+proof -
+  assume "typecheck' \<Gamma> vs e = (e', t, vs', con)"
+  hence "quick_convert vs e = (e', vs')" by simp
+  thus ?thesis by simp
+qed
 
 lemma [simp]: "tree_code_size_list cd = code_list_size (tco_cd cd)"
   by (induction cd rule: tco_cd.induct) (simp_all split: list.splits)
@@ -51,7 +101,10 @@ lemma [simp]: "tree_code_size_list cd = code_list_size (tco_cd cd)"
 lemma [simp]: "alg_compile2 lib cd acc = flatten_code' lib (tco_cd cd) (tco_r cd) @ acc"
   by (induction lib cd acc rule: alg_compile2.induct) simp_all
 
-lemma [simp]: "alg_compile = flatten_code \<circ> tco \<circ> encode \<circ> convert"
-  by rule (simp add: alg_compile_def convert_def tco_def)
+lemma [simp]: "collect_constraints \<Gamma> vs e = snd (typecheck' \<Gamma> vs e)"
+  by (induction e arbitrary: \<Gamma> vs) (simp_all add: Let_def split: option.splits prod.splits)
+
+lemma [simp]: "alg_compile = map_option (flatten_code \<circ> tco \<circ> encode \<circ> convert \<circ> fst) \<circ> typecheck"
+  by rule (auto simp add: alg_compile_def convert_def tco_def split: prod.splits option.splits)
 
 end
